lambda2Gmu/Infrastructure.v
@@ -1492,3 +1492,32 @@ Lemma subst_te_many_commutes_open : forall As Ts e x,
     f_equal.
     apply subst_te_open_ee_var.
 Qed.
+
+Lemma fv_env_extend : forall E x T,
+    fv_env (E & x ~: T) = fv_typ T \u fv_env E.
+  intros.
+  rewrite concat_def.
+  rewrite single_def.
+  cbn.
+  fold (fv_env E).
+  trivial.
+Qed.
+
+Lemma notin_env_inv : forall E X x T,
+    X \notin fv_env (E & x ~: T) ->
+    X \notin fv_env E /\ X \notin fv_typ T.
+  introv Fr.
+  rewrite fv_env_extend in Fr.
+  rewrite* notin_union in Fr.
+Qed.
+
+Lemma notin_domΔ_eq : forall D1 D2 X,
+    X \notin domΔ (D1 |,| D2) <->
+    X \notin domΔ D1 /\ X \notin domΔ D2.
+  induction D1; intros; constructor;
+    try solve [cbn in *; intuition]; intro H;
+      destruct a; cbn in *;
+        repeat rewrite notin_union in *;
+        destruct (IHD1 D2 X) as [IH1 IH2];
+        intuition.
+Qed.
